PolyLoopSimpl.v
@@ -1,0 +1,76 @@
+Require Import ZArith.
+Require Import List.
+Require Import Bool.
+Require Import Psatz.
+
+Require Import Linalg.
+Require Import Misc.
+Require Import Semantics.
+Require Import PolyLoop.
+Require Import PolyOperations.
+Require Import ImpureAlarmConfig.
+
+Open Scope Z_scope.
+
+Fixpoint polyloop_simplify stmt n ctx :=
+  match stmt with
+  | PSkip => pure PSkip
+  | PSeq st1 st2 => BIND s1 <- polyloop_simplify st1 n ctx -; BIND s2 <- polyloop_simplify st2 n ctx -; pure (PSeq s1 s2)
+  | PGuard pol st =>
+    let pol := resize_poly n pol in
+    BIND npol <- ctx_simplify pol ctx -;
+    BIND nctx <- poly_inter pol ctx -;
+    BIND nst <- polyloop_simplify st n nctx -;
+    pure (PGuard npol nst)
+  | PLoop pol st =>
+    let pol := resize_poly (S n) pol in
+    BIND npol <- ctx_simplify pol ctx -;
+    BIND nctx <- poly_inter pol ctx -;
+    BIND nst <- polyloop_simplify st (S n) nctx -;
+    pure (PLoop npol nst)
+  | PInstr i es => pure (PInstr i es)
+  end.
+
+Lemma polyloop_simplify_correct :
+  forall stmt n ctx,
+    (poly_nrl ctx <= n)%nat ->
+    WHEN nst <- polyloop_simplify stmt n ctx THEN
+         forall env mem1 mem2, length env = n -> in_poly (rev env) ctx = true ->
+                          poly_loop_semantics nst env mem1 mem2 ->
+                          poly_loop_semantics stmt env mem1 mem2.
+Proof.
+  induction stmt; intros n ctx Hctx nst Hnst env mem1 mem2 Henvlen Henvctx Hsem; simpl in *.
+  - bind_imp_destruct Hnst npol Hnpol; bind_imp_destruct Hnst nctx Hnctx.
+    bind_imp_destruct Hnst nst1 Hnst1; apply mayReturn_pure in Hnst; rewrite <- Hnst in *.
+    apply PLLoop_inv_sem in Hsem.
+    assert (Hinctx : forall x, in_poly (rev (x :: env)) ctx = true) by
+        (intros x; rewrite <- in_poly_nrlength with (n := n); [|auto]; simpl; rewrite resize_app by (rewrite rev_length; auto); auto).
+    assert (Heq : forall x, in_poly (rev (x :: env)) npol = in_poly (rev (x :: env)) p) by
+        (intros x; erewrite <- (ctx_simplify_correct _ _ _ Hnpol); [rewrite resize_poly_in; [|rewrite rev_length]; simpl; auto|auto]).
+    destruct Hsem as [lb [ub [Hlbub Hsem]]].
+    apply PLLoop with (lb := lb) (ub := ub); [intros x; rewrite <- Heq; apply Hlbub|].
+    eapply iter_semantics_map; [|exact Hsem].
+    intros x mem3 mem4 Hx Hsem1. simpl in *.
+    rewrite Zrange_in, <- Hlbub, Heq in Hx.
+    assert (Hnctxnrl : (poly_nrl nctx <= S n)%nat) by (eapply poly_inter_nrl; [apply resize_poly_nrl| |exact Hnctx]; lia).
+    eapply IHstmt; [exact Hnctxnrl|exact Hnst1|simpl; auto| |exact Hsem1].
+    erewrite poly_inter_def, poly_inter_pure_def, resize_poly_in; [|rewrite rev_length|exact Hnctx]; [|simpl; auto]; reflect; simpl; auto.
+  - apply mayReturn_pure in Hnst; rewrite <- Hnst in *; auto.
+  - apply mayReturn_pure in Hnst; rewrite <- Hnst in *; auto.
+  - bind_imp_destruct Hnst s1 Hs1; bind_imp_destruct Hnst s2 Hs2; apply mayReturn_pure in Hnst; rewrite <- Hnst in *.
+    apply PLSeq_inv_sem in Hsem; destruct Hsem as [mem3 [Hsem1 Hsem2]].
+    apply PLSeq with (mem2 := mem3); [eapply IHstmt1 | eapply IHstmt2]; eauto.
+  - bind_imp_destruct Hnst npol Hnpol; bind_imp_destruct Hnst nctx Hnctx.
+    bind_imp_destruct Hnst nst1 Hnst1; apply mayReturn_pure in Hnst; rewrite <- Hnst in *.
+    apply PLGuard_inv_sem in Hsem.
+    replace (in_poly (rev env) npol) with (in_poly (rev env) p) in *.
+    + destruct (in_poly (rev env) p) eqn:Hin.
+      * apply PLGuardTrue; [|auto].
+        assert (Henvnctx : in_poly (rev env) nctx = true) by
+            (erewrite poly_inter_def, poly_inter_pure_def; [|exact Hnctx]; reflect; rewrite resize_poly_in; auto; rewrite rev_length; auto).
+        assert (Hnctxnrl : (poly_nrl nctx <= n)%nat) by (eapply poly_inter_nrl; [apply resize_poly_nrl|exact Hctx|exact Hnctx]).
+        eapply IHstmt with (n := n) (ctx := nctx); eauto.
+      * rewrite Hsem. apply PLGuardFalse; auto.
+    + erewrite <- (ctx_simplify_correct _ _ _ Hnpol); auto.
+      rewrite resize_poly_in; [|rewrite rev_length]; auto.
+Qed.
